Logic/Propositional/Superintuitionistic/Deduction.lean
@@ -8,43 +8,43 @@ variable {α : Type u} [DecidableEq α]
 
 structure DeductionParameter (α) where
   axiomSet : AxiomSet α
-notation "Ax(" 𝓓 ")" => DeductionParameter.axiomSet 𝓓
+notation "Ax(" Λ ")" => DeductionParameter.axiomSet Λ
 
 namespace DeductionParameter
 
-class IncludeEFQ (𝓓 : DeductionParameter α) where
-  include_EFQ : 𝗘𝗙𝗤 ⊆ Ax(𝓓) := by simp
+class IncludeEFQ (Λ : DeductionParameter α) where
+  include_EFQ : 𝗘𝗙𝗤 ⊆ Ax(Λ) := by simp
 
-class IncludeLEM (𝓓 : DeductionParameter α) where
-  include_LEM : 𝗟𝗘𝗠 ⊆ Ax(𝓓) := by simp
+class IncludeLEM (Λ : DeductionParameter α) where
+  include_LEM : 𝗟𝗘𝗠 ⊆ Ax(Λ) := by simp
 
-class IncludeDNE (𝓓 : DeductionParameter α) where
-  include_DNE : 𝗗𝗡𝗘 ⊆ Ax(𝓓) := by simp
+class IncludeDNE (Λ : DeductionParameter α) where
+  include_DNE : 𝗗𝗡𝗘 ⊆ Ax(Λ) := by simp
 
 end DeductionParameter
 
-inductive Deduction (𝓓 : DeductionParameter α) : Formula α → Type _
-  | eaxm {p}     : p ∈ Ax(𝓓) → Deduction 𝓓 p
-  | mdp {p q}    : Deduction 𝓓 (p ⟶ q) → Deduction 𝓓 p → Deduction 𝓓 q
-  | verum        : Deduction 𝓓 $ ⊤
-  | imply₁ p q   : Deduction 𝓓 $ p ⟶ q ⟶ p
-  | imply₂ p q r : Deduction 𝓓 $ (p ⟶ q ⟶ r) ⟶ (p ⟶ q) ⟶ p ⟶ r
-  | and₁ p q     : Deduction 𝓓 $ p ⋏ q ⟶ p
-  | and₂ p q     : Deduction 𝓓 $ p ⋏ q ⟶ q
-  | and₃ p q     : Deduction 𝓓 $ p ⟶ q ⟶ p ⋏ q
-  | or₁ p q      : Deduction 𝓓 $ p ⟶ p ⋎ q
-  | or₂ p q      : Deduction 𝓓 $ q ⟶ p ⋎ q
-  | or₃ p q r    : Deduction 𝓓 $ (p ⟶ r) ⟶ (q ⟶ r) ⟶ (p ⋎ q ⟶ r)
-  | neg_equiv p  : Deduction 𝓓 $ Axioms.NegEquiv p
+inductive Deduction (Λ : DeductionParameter α) : Formula α → Type _
+  | eaxm {p}     : p ∈ Ax(Λ) → Deduction Λ p
+  | mdp {p q}    : Deduction Λ (p ⟶ q) → Deduction Λ p → Deduction Λ q
+  | verum        : Deduction Λ $ ⊤
+  | imply₁ p q   : Deduction Λ $ p ⟶ q ⟶ p
+  | imply₂ p q r : Deduction Λ $ (p ⟶ q ⟶ r) ⟶ (p ⟶ q) ⟶ p ⟶ r
+  | and₁ p q     : Deduction Λ $ p ⋏ q ⟶ p
+  | and₂ p q     : Deduction Λ $ p ⋏ q ⟶ q
+  | and₃ p q     : Deduction Λ $ p ⟶ q ⟶ p ⋏ q
+  | or₁ p q      : Deduction Λ $ p ⟶ p ⋎ q
+  | or₂ p q      : Deduction Λ $ q ⟶ p ⋎ q
+  | or₃ p q r    : Deduction Λ $ (p ⟶ r) ⟶ (q ⟶ r) ⟶ (p ⋎ q ⟶ r)
+  | neg_equiv p  : Deduction Λ $ Axioms.NegEquiv p
 
 instance : System (Formula α) (DeductionParameter α) := ⟨Deduction⟩
 
 open Deduction
 open DeductionParameter
 
-variable {𝓓 : DeductionParameter α}
+variable {Λ : DeductionParameter α}
 
-instance : System.Minimal 𝓓 where
+instance : System.Minimal Λ where
   mdp := mdp
   verum := verum
   imply₁ := imply₁
@@ -57,25 +57,25 @@ instance : System.Minimal 𝓓 where
   or₃ := or₃
   neg_equiv := neg_equiv
 
-instance [𝓓.IncludeEFQ] : System.HasAxiomEFQ 𝓓 where
+instance [Λ.IncludeEFQ] : System.HasAxiomEFQ Λ where
   efq _ := eaxm $ Set.mem_of_subset_of_mem IncludeEFQ.include_EFQ (by simp);
 
-instance [𝓓.IncludeLEM] : System.HasAxiomLEM 𝓓 where
+instance [Λ.IncludeLEM] : System.HasAxiomLEM Λ where
   lem _ := eaxm $ Set.mem_of_subset_of_mem IncludeLEM.include_LEM (by simp);
 
-instance [𝓓.IncludeDNE] : System.HasAxiomDNE 𝓓 where
+instance [Λ.IncludeDNE] : System.HasAxiomDNE Λ where
   dne _ := eaxm $ Set.mem_of_subset_of_mem IncludeDNE.include_DNE (by simp);
 
-instance [𝓓.IncludeEFQ] : System.Intuitionistic 𝓓 where
+instance [Λ.IncludeEFQ] : System.Intuitionistic Λ where
 
-instance [𝓓.IncludeDNE] : System.Classical 𝓓 where
+instance [Λ.IncludeDNE] : System.Classical Λ where
 
-instance [𝓓.IncludeEFQ] [𝓓.IncludeLEM] : System.Classical 𝓓 where
+instance [Λ.IncludeEFQ] [Λ.IncludeLEM] : System.Classical Λ where
 
 
 namespace DeductionParameter
 
-lemma eaxm! {𝓓 : DeductionParameter α} {p : Formula α} (h : p ∈ Ax(𝓓)) : 𝓓 ⊢! p := ⟨eaxm h⟩
+lemma eaxm! {Λ : DeductionParameter α} {p : Formula α} (h : p ∈ Ax(Λ)) : Λ ⊢! p := ⟨eaxm h⟩
 
 protected abbrev Minimal : DeductionParameter α := { axiomSet := ∅ }
 
@@ -122,10 +122,10 @@ variable {Λ : DeductionParameter α}
 
 open System
 
-noncomputable def rec! {α : Type u} {𝓓 : DeductionParameter α}
-  {motive : (a : Formula α) → 𝓓 ⊢! a → Sort u_1}
-  (eaxm   : ∀ {p}, (a : p ∈ Ax(𝓓)) → motive p ⟨eaxm a⟩)
-  (mdp    : ∀ {p q}, {hpq : 𝓓 ⊢! (p ⟶ q)} → {hp : 𝓓 ⊢! p} → motive (p ⟶ q) hpq → motive p hp → motive q (hpq ⨀ hp))
+noncomputable def rec! {α : Type u} {Λ : DeductionParameter α}
+  {motive : (a : Formula α) → Λ ⊢! a → Sort u_1}
+  (eaxm   : ∀ {p}, (a : p ∈ Ax(Λ)) → motive p ⟨eaxm a⟩)
+  (mdp    : ∀ {p q}, {hpq : Λ ⊢! (p ⟶ q)} → {hp : Λ ⊢! p} → motive (p ⟶ q) hpq → motive p hp → motive q (hpq ⨀ hp))
   (verum  : motive ⊤ verum!)
   (imply₁ : ∀ {p q},   motive (p ⟶ q ⟶ p) imply₁!)
   (imply₂ : ∀ {p q r}, motive ((p ⟶ q ⟶ r) ⟶ (p ⟶ q) ⟶ p ⟶ r) imply₂!)
@@ -136,7 +136,7 @@ noncomputable def rec! {α : Type u} {𝓓 : DeductionParameter α}
   (or₂    : ∀ {p q},   motive (q ⟶ p ⋎ q) or₂!)
   (or₃    : ∀ {p q r}, motive ((p ⟶ r) ⟶ (q ⟶ r) ⟶ p ⋎ q ⟶ r) or₃!)
   (neg_equiv : ∀ {p}, motive (Axioms.NegEquiv p) neg_equiv!) :
-  {a : Formula α} → (t : 𝓓 ⊢! a) → motive a t := by
+  {a : Formula α} → (t : Λ ⊢! a) → motive a t := by
   intro p d;
   induction d.some with
   | eaxm h => exact eaxm h
