Logic/Modal/Standard/Kripke/Kripke.lean
@@ -1,4 +1,3 @@
-import Logic.Modal.Standard.Kripke.Soundness
 import Logic.Modal.Standard.Kripke.Completeness
 import Logic.Modal.Standard.Kripke.Preservation
 import Logic.Modal.Standard.Kripke.Filteration
